examples/map/MapIAproof.v
@@ -1,19 +1,21 @@
 Require Import CRIS.
 
-Require Import MapHeader MapA MapM MapI ModSim MapIMproof MapMAproof MemA.
+Require Import MapHeader MapA MapM MapI ModSim MapIMproof MapMAproof MemA wpsim.
 
 Module MapIA. Section MapIA.
   Context `{!invG α Σ Γ, !subG Γ Σ, !sinvG Σ Γ α β τ, !MapAGΓ Γ, !MapMGΓ Γ, !memGΓ Γ}.
+  Context (υ : univ_id) (n : level).
+  Context `((υ > 2)%positive).
 
   Theorem correct gi (SpcMap SpcMem : string → option fspec)
-      (MapInSpcMap : spc_incl MapAS.Spc SpcMap) :
+      (MapInSpcMap : spc_incl (MapAS.Spc υ n) SpcMap) :
     ctx_refines
-      ((MapA.t gi SpcMap)  ★ (MemA.t gi SpcMem), (MapA.InitCond ∗ MapM.InitCond)%I)
-      ((MapI.t)            ★ (MemA.t gi SpcMem), emp%I).
+      ((MapA.t υ n gi SpcMap)  ★ (MemA.t gi SpcMem), (MapA.InitCond ∗ MapM.InitCond)%I)
+      ((MapI.t)                ★ (MemA.t gi SpcMem), emp%I).
   Proof.
     etrans; cycle 1.
     { eapply main_adequacy. eapply MapIM.sim.
-      instantiate (1:= to_spc MapMS.Spc).
+      instantiate (1:= to_spc (MapMS.Spc 1%positive n)).
       i. split; try refl. unfold MapMS.Spc. unseal CRIS. prove_nodup.
     }
     etrans; cycle 1.
@@ -24,5 +26,34 @@ Module MapIA. Section MapIA.
       rewrite /MapMS.Spc; unseal CRIS; prove_nodup.
     }
     refl.
+  Unshelve. r; lia.
   Qed.
 End MapIA. End MapIA.
+
+Module w_MapIA. Section w_MapIA.
+  Context `{!invG α Σ Γ, !subG Γ Σ, !sinvG Σ Γ α β τ, !MapAGΓ Γ, !MapMGΓ Γ, !memGΓ Γ}.
+  Context (n : level).
+  Theorem correct gi (SpcMap : univ_id → string → option fspec) (SpcMem : string → option fspec)
+      (MapInSpcMap : ∀ υ, spc_incl (MapAS.Spc υ n) (SpcMap υ)) :
+    w_ctx_refines
+      (λ υ, ((MapA.t υ n gi (SpcMap υ))  ★ (MemA.t gi SpcMem), (MapA.InitCond ∗ MapM.InitCond)%I))
+      (λ _, ((MapI.t)                    ★ (MemA.t gi SpcMem), emp%I)).
+  Proof.
+    etrans; cycle 1.
+    { eapply MapIMproof.wctxr.
+      instantiate (1:= λ u, to_spc (MapMS.Spc u%positive n)).
+      i. split; try refl. unfold MapMS.Spc. unseal CRIS. prove_nodup.
+    }
+    etrans; cycle 1.
+    { eapply w_ctx_refines_frameR.
+      instantiate (1:=(λ υ, emp%I ∗ MapM.InitCond)%I).
+      eapply w_ctx_refines_cond_frameR.
+      (* rewrite -(hmod_addc_empty_l _ MapM.InitCond). *)
+      eapply ctxr_cond_frameR, main_adequacy, MapMA.sim; eauto.
+      split; try refl.
+      rewrite /MapMS.Spc; unseal CRIS; prove_nodup.
+    }
+    refl.
+  Unshelve. r; lia.
+  Qed.
+End w_MapIA. End w_MapIA.
