examples/map/MapMAproof.v
@@ -177,3 +177,18 @@ Module MapMA. Section MapMA.
     - apply simF_set_by_user; eauto.
   Qed.
 End MapMA. End MapMA.
+(* 
+Section wctxr.
+  Context `{!invG α Σ Γ, !subG Γ Σ, !sinvG Σ Γ α β τ, !MapAGΓ Γ, !MapMGΓ Γ, !memGΓ Γ}.
+  Lemma wctxr n Spc_s Spc_t ginv_t ginv_s
+      (MapInSpcS : ∀ υ, spc_incl (MapAS.Spc υ n) (Spc_s υ))
+      (MapInSpcT : ∀ υ, spc_incl (MapMS.Spc υ n) (Spc_t υ)) :
+    w_ctx_refines
+      (λ υ, ((MapA.t υ n ginv_s (Spc_s υ)), MapA.InitCond))
+      (λ ν, (MapM.t ν n ginv_t (Spc_t ν), emp%I)).
+  Proof.
+    exists 1; move => u v Huv; eapply main_adequacy with (Ist := MapMA.Ist).
+    assert (ModRel u v). { r. lia. }
+    eapply MapMA.sim; eauto.
+  Qed.
+End wctxr. *)
